theories/Plugin.v
@@ -1,13 +1,22 @@
 Require Import Utils.
 Require Import Vector.
 Require Import Circuit.
-Require Import NativeCircuit.
 
 Require Coq.Lists.List.
 Import List.ListNotations.
 
 Register le_S as num.nat.le_S.
 Register length as core.list.length.
+
+Lemma prove_nat_le :
+  forall n m,
+  PeanoNat.Nat.leb n m = true ->
+  n <= m.
+Proof.
+  intros n m H. rewrite (Bool.reflect_iff _ _ (PeanoNat.Nat.leb_spec0 n m)). auto.
+Qed.
+
+Register prove_nat_le as num.nat.prove_le.
 
 Fixpoint bitlist_to_nat (bl : list bool) : nat :=
   match bl with
@@ -22,35 +31,5 @@ Fixpoint bitlist_of_nat (n m : nat) : list bool :=
   | 0 => []
   | S n' => (Nat.eqb (Nat.modulo m 2) 1) :: bitlist_of_nat n' (Nat.div m 2)
   end.
-
-Lemma prove_eq :
-  forall n m,
-  PeanoNat.Nat.eqb n m = true ->
-  n = m.
-Proof.
-  intros n m H. rewrite (Bool.reflect_iff _ _ (PeanoNat.Nat.eqb_spec n m)). auto.
-Qed.
-
-Register prove_eq as vcpu.prove_eq.
-
-Lemma prove_le :
-  forall n m,
-  PeanoNat.Nat.leb n m = true ->
-  n <= m.
-Proof.
-  intros n m H. rewrite (Bool.reflect_iff _ _ (PeanoNat.Nat.leb_spec0 n m)). auto.
-Qed.
-
-Register prove_le as vcpu.prove_le.
-
-Lemma prove_le_fast :
-  forall n m,
-  n <= m.
-Proof.
-Admitted.
-
-Register prove_le_fast as vcpu.prove_le_fast.
-
-Register int as int.
 
 Declare ML Module "vcpu_plugin:vcpu-plugin.plugin".
